tenative at translation correction

theories/mcalc/DCtoLC.v
@@ -102,7 +102,6 @@ Require Import MySequences.
 Require Import DCReduction.
 
 
-
 Theorem safe_optimization:
   forall t Delta,
   is_pure (pure .: Delta) t = pure ->
@@ -117,377 +116,8 @@ Proof.
   The first reduces to [Lam y. Empty], while the second one reduces to [Empty]. Both terms are terminals.
   ".
 Abort.
-  
-
-(** translation correction *)
-
-Require Import STDCDefinition.
-Module DT := STDCDefinition.
-Module LT := STLCDefinition.
-
-Module DVR := DCValuesRes.
-
-Require Import Program.
 
 
-Fixpoint trans_ty_aux ty := 
-  match ty with
-  | DT.TyVar x => LT.TyVar x 
-  | DT.TyFun A B => LT.TyFun (trans_ty_aux A) (LT.TyOption (trans_ty_aux B))
-  | DT.TyBool => LT.TyBool
-  end.
-
-Definition trans_ty (b: bool) ty := if b then trans_ty_aux ty else LT.TyOption (trans_ty_aux ty).
-(* 
-Lemma jt_te_thunk Gamma t tau:
-  LT.jt Gamma t tau ->
-  forall u,
-  LT.jt Gamma (thunk t) (LT.TyFun u tau).
-Proof.
-  unfold thunk.
-  intros.
-  econstructor.
-  now eapply jt_te_renaming_0.
-Qed. *)
-
-
-Lemma trans_correct_type Gamma t1 tau:
-  jt Gamma t1 tau ->
-  forall Delta,
-  LT.jt (fun x => trans_ty (Delta x) (Gamma x)) (trans Delta t1) (trans_ty false tau).
-Proof.
-  induction 1 using jt_ind'; intros; try solve [simpl; eauto with jt].
-  * remember (Delta x) as b.
-    induction b; simpl; symmetry in Heqb; rewrite Heqb.
-    - repeat econstructor; rewrite Heqb, H; eauto.
-    - repeat econstructor; rewrite Heqb, H; eauto.
-  * simpl.
-    repeat econstructor.
-    replace (trans_ty_aux T .: (fun x : var => trans_ty (Delta x) (Gamma x))) with (fun x : var => trans_ty ((true .: Delta) x) ((T .: Gamma) x)).
-    eapply IHjt.
-    { unfold ".:".
-      eapply functional_extensionality.
-      intros; induction x; simpl; eauto.
-    }
-  * simpl trans.
-    induction t1; try solve [repeat econstructor|
-    (* general case *)
-    repeat eapply JTmonad_bind;
-    solve
-      [ eapply IHjt1
-      | eapply jt_te_renaming_0;eapply IHjt2
-      | repeat econstructor ]
-    ].
-    (* We consider all the cases for App. *)
-    - (* First case : App (Var x) _. Either Delta x is true or false. *)
-      remember (Delta x) as b.
-      induction b; symmetry in Heqb.
-      + (* If Delta x is true, *)
-        eapply JTmonad_bind.
-        { apply IHjt2. }
-        { inverts H. repeat econstructor. asimpl.
-          rewrite Heqb, H3. now asimpl. } 
-      + (* If Delta x is false *)
-        eapply JTmonad_bind.
-        { simpl in IHjt1.
-          specialize IHjt1 with Delta.
-          rewrite Heqb in IHjt1.
-          apply IHjt1.
-        }
-        { eapply JTmonad_bind; repeat econstructor.
-          { simpl in IHjt2.
-            eapply jt_te_renaming_0.
-            eapply IHjt2. }
-        }
-    - (* Second case: [App (Lam body) arg] represents an [let arg in body] statement. *)
-      eapply JTmonad_bind.
-      { eapply IHjt2. }
-      { 
-        inverts H.
-        specialize IHjt1 with ((* true .: *) Delta).
-        simpl in IHjt1.
-        inverts IHjt1.
-        inverts H3.
-        eapply H5.
-      }
-  * simpl. 
-    rename H0 into IHjts.
-    eapply JTmonad_handle.
-    - induction ts. { econstructor. }
-      simpl.
-      inverts_Forall.
-      econstructor; eauto.
-    - simpl in *. eapply IHjt1.
-    - simpl in *. eapply IHjt2.
-Qed.
-
-(* TODO : look at the trans definition when App does not have multiple arguments. *)
-
-Require Import FunInd.
-
-
-(******************************************************************************)
-
-
-
-Section SUBSTITUTION.
-
-(* The goal of this part is to prove a substitution lemma for trans *)
-
-Lemma trans_te_renaming:
-  forall Delta t u,
-  trans Delta t = u ->
-  forall Delta' xi,
-  Delta = xi >>> Delta' ->
-  trans Delta' t.[ren xi] = u.[ren xi].
-Proof.
-  intros Delta t u Hu.
-  subst.
-  gen Delta.
-  induction t using term_ind'; intros; subst;
-  try solve [asimpl; unfold_monad;
-  eauto with autosubst].
-  * (* Case [Var x]. We just need to look at [Delta x]. *)
-    simpl; unfold_monad.
-    case (Delta' (xi x)); eauto with autosubst.
-  * (* Case [Lam _] nothing particular. *)
-    asimpl; unfold_monad; repeat f_equal; eauto with autosubst.
-  * (* Case [App _ _] *)
-    
-    remember t1; induction t1; subst; try eauto with autosubst.
-    - (* Case [App (Var f) _ ]*)
-      intros; subst.
-      simpl trans.
-      case (Delta' (xi x)).
-      + unfold_monad.
-        rewrite
-          subst_match,
-          subst_variant_none,
-          subst_app,
-          subst_var.
-        repeat f_equal.
-        eapply IHt2; reflexivity.
-      + unfold_monad. 
-        repeat rewrite
-          subst_match,
-          subst_match,
-          subst_app,
-          subst_variant_none,
-          subst_var.
-        do 2 f_equal.
-        erewrite IHt2; try reflexivity.
-        rewrite lift_up; tc.
-    - (* Case [App (Lam _) _]*)
-      intros; clear IHt0.
-      Opaque trans. asimpl. Transparent trans.
-      simpl trans.
-      unfold_monad.
-      asimpl.
-      unfold monad_return in IHt1.
-      f_equal.
-      + eapply IHt2; eauto.
-      + simpl trans in IHt1.
-        assert (trans Delta' (Lam t0).[ren xi] = (trans (xi >>> Delta') (Lam t0)).[ren xi]).
-        { unfold monad_return in IHt1. forwards: IHt1 (xi >>> Delta') Delta' xi; eauto. }
-        injections. eauto with autosubst.
-  * asimpl.
-    rewrite subst_monad_handle.
-    f_equal; eauto.
-    { induction ts; asimpl; inverts_Forall; repeat f_equal; eauto. }
-Qed.
-
-Lemma trans_te_renaming_0:
-  forall Gamma t T u,
-  trans Gamma t = u ->
-  trans (T .: Gamma) (lift 1 t) = (lift 1 u).
-Proof.
-  intros.
-  eapply trans_te_renaming; eauto.
-Qed.
-
-Hypothesis iota_equality: forall t1 t2,
-  (* match Some t1 with None => None | Some x => t2  = t2.[x |-> t1] *)
-  EMatch (EVariantSome t1) EVariantNone t2 = t2.[t1/].
-
-Hypothesis eta_equality: forall t1 t2,
-  EApp (ELam t1) t2 = t1.[t2/].
-
-Theorem trans_te_substitution:
-  forall t Delta,
-  forall sigma1 sigma2,
-  (exists Gamma T, jt Gamma t T) ->
-  (exists Gamma T, jt Gamma t.[sigma1] T) ->
-  (forall x, is_value_res (sigma1 x) \/ (sigma1 x) = ids x) ->
-  (forall x, is_nerror (sigma1 x)) ->
-  (forall x, Delta x = true -> (trans Delta (sigma1 x)) = EVariantSome (sigma2 x)) ->
-  (forall x, Delta x = false -> (trans Delta (sigma1 x)) = sigma2 x) ->
-  trans Delta t.[sigma1] = (trans Delta t).[sigma2].
-Proof.
-  induction t using term_ind'; try eauto.
-  3: {
-    introv [Gamma [T Hty]] [Gamma' [T' Hty']] Hval Hnerr HsigmaT HsigmaF.
-    induction t1; try solve [asimpl; eauto].
-    - (* Case [App (Var x) _] *) 
-      assert (Hvalx: is_value_res (sigma1 x) \/ sigma1 x = ids x) by eapply Hval.
-      assert (Hnerrx: is_nerror (sigma1 x)) by eapply Hnerr.
-      asimpl; remember (sigma1 x) as t; induction t; try clear IHt; destruct Hvalx; tryfalse; injections; subst.
-      {
-        asimpl.
-        remember (Delta x).
-        induction b; asimpl; unfold_monad; fequal.
-        { 
-          inverts Hty; inverts Hty'.
-          eapply IHt2; eauto.
-        }
-        { fequal. assert (H: trans Delta (sigma1 x) = EVariantSome (sigma2 x)).
-          { eapply HsigmaT; eauto. }
-          rewrite <- Heqt in H; asimpl in H; rewrite <- Heqb in H; unfold monad_return in H.
-          injections.
-          rewrite <- H; eauto.
-        }
-        { fequal. assert (H: trans Delta (sigma1 x) = sigma2 x).
-          { eapply HsigmaF; eauto. }
-          rewrite <- Heqt in H; asimpl in H; rewrite <- Heqb in H; unfold monad_return in H.
-          eauto.
-        }
-        { f_equal.
-          inverts Hty; inverts Hty'.
-          erewrite IHt2; eauto; asimpl.
-          eauto.
-        }
-      }
-      {
-        asimpl.
-        remember (Delta x).
-        induction b; asimpl; unfold_monad.
-        - inverts Hty; inverts Hty'.
-          erewrite IHt2; eauto.
-          replace (sigma2 x) with (L.ELam (trans (true .: Delta) t)).
-          { asimpl; repeat f_equal.
-            rewrite eta_equality; asimpl; eauto.
-          }
-          {
-            symmetry in Heqb.
-            assert (Hsigma: trans Delta (sigma1 x) = EVariantSome (sigma2 x)) by eauto.
-            rewrite <- Heqt in Hsigma. simpl in Hsigma. unfold monad_return in Hsigma.
-            injections; eauto.
-          }
-        - erewrite IHt2; eauto.
-          2:{ inverts Hty; eauto. }
-          2:{ inverts Hty'; eauto. }
-
-          erewrite <- HsigmaF; eauto. rewrite <- Heqt. asimpl; unfold_monad.
-          rewrite iota_equality; asimpl.
-          rewrite eta_equality; asimpl.
-          repeat f_equal.
-      }
-      { (* Then x has type bool, and this is not possible since it must have type TyArrow.*)
-          false.
-          inverts Hty'.
-          match goal with [h: jt _ (sigma1 x) (TyFun _ _) |- _] =>
-            rewrite <- Heqt in h;
-            inverts h
-          end.
-        }
-    - (* Case [App (Lam t) _ ] *)
-      asimpl; unfold_monad.
-      
-      repeat f_equal.
-      * (* by IHt2, [trans Delta t2.[sigma1] = (trans Delta t2).[sigma2]] *)
-        erewrite IHt2; eauto.
-        { inverts Hty. inverts Hty'. exists Gamma T0. eauto. }
-        { inverts Hty. inverts Hty'. exists Gamma' T1. eauto. }
-      * (* by IHt1, [trans Delta (Lam t).[sigma1] = (trans Delta (Lam t)).[sigma2]]. *)
-        assert (trans Delta (Lam t).[sigma1] = (trans Delta (Lam t)).[sigma2]).
-        { eapply IHt1; eauto; inverts Hty; inverts Hty'.
-          { exists Gamma (TyFun T0 T); eauto. }
-          { exists Gamma' (TyFun T1 T'); eauto. }
-        }
-        asimpl in H.
-        injections; eauto.
-  }
-  3: {
-    introv [Gamma [T Hty]] [Gamma' [T' Hty']] Hval Hnerr HsigmaT HsigmaF.
-    assert (Hts: List.map (trans Delta) ts..[sigma1] = (List.map (trans Delta) ts)..[sigma2]).
-    { induction ts; asimpl; repeat f_equal.
-      - inverts Hty; inverts Hty'. inverts_Forall.
-        eapply H4; eauto.
-      - inverts Hty; inverts Hty'. inverts_Forall.
-        eapply IHts; eauto using jt. 
-    }
-    assert (Ht1: trans Delta t1.[sigma1] = (trans Delta t1).[sigma2]).
-    { 
-      eapply IHt1; eauto.
-      inverts Hty; exists Gamma TyBool; eauto.
-      inverts Hty'; exists Gamma' TyBool; eauto.
-    }
-    assert (Ht2: trans Delta t2.[sigma1] = (trans Delta t2).[sigma2]).
-    { eapply IHt2; eauto.
-      inverts Hty; exists Gamma T; eauto.
-      inverts Hty'; exists Gamma' T'; eauto.
-    }
-
-    asimpl.
-    rewrite Hts, Ht1, Ht2.
-    rewrite subst_monad_handle.
-    eauto.
-  }
-  2: {
-    (* Case [Lam _] *)
-    introv [Gamma [T Hty]] [Gamma' [T' Hty']] Hval Hnerr HsigmaT HsigmaF.
-    asimpl.
-    unfold_monad. repeat fequal.
-    inverts Hty; inverts Hty'.
-    eapply IHt; eauto.
-    - induction x.
-      * asimpl; eauto.
-      * destruct (Hval x) as [H|H].
-        { left; asimpl; eapply is_value_res_renaming; eauto. }
-        { right; asimpl. rewrite H; eauto. }
-    - clear -Hnerr.
-      induction x; asimpl.
-      { unfold ids, D.Ids_term; eauto. }
-      { specialize Hnerr with x.
-        remember (sigma1 x) as t.
-        induction t; asimpl; eauto.
-      }
-    - clear -HsigmaT.
-      induction x; intros.
-      { unfold ids, D.Ids_term; asimpl; eauto. }
-      { asimpl.
-        replace (EVariantSome (lift 1 (sigma2 x))) with (lift 1 (EVariantSome (sigma2 x))); eauto using trans_te_renaming_0. }
-    - clear -HsigmaF.
-      induction x; asimpl; intros.
-      { tryfalse. }
-      { eapply trans_te_renaming_0; eauto. }
-  }
-  { (* case [Var _] *)
-    introv [Gamma [T Hty]] [Gamma' [T' Hty']] Hval Hnerr HsigmaT HsigmaF.
-    asimpl.
-    remember (Delta x) as b.
-    specialize HsigmaT with x.
-    specialize HsigmaF with x.
-    induction b; eauto.
-  }
-Qed.
-
-Lemma trans_te_substitution_0:
-  forall b Delta t1 t2,
-  (exists (Gamma : tyenv) (T : ty), jt Gamma t1 T) ->
-  (exists (Gamma : tyenv) (T : ty), jt Gamma t1.[t2/] T) ->
-  is_value_res t2 ->
-  is_nerror t2 ->
-  trans (b .: Delta) t1.[t2/] = (trans (b .: Delta) t1).[(trans (b .: Delta) t2)/].
-Proof.
-  intros.
-  eapply trans_te_substitution; eauto.
-  {
-    induction x; simpl; eauto.
-  }
-
-Abort.
-
-End SUBSTITUTION.
 
 Section Correctness.
 
@@ -560,46 +190,186 @@ Tactic Notation "save" uconstr(E) "as" ident(x) :=
   match goal with [ h: context [E] |- _ ] => rename h into x end.
 
 
+Require Import STDCDefinition.
+
+Lemma trans_is_value Delta v:
+  is_value v -> LCValues.is_value (trans Delta v).
+Admitted.
+
+Lemma trans_subst_pure Delta t v:
+  pure = is_pure Delta v ->
+  exists target,
+    star lcbv (trans (pure .: Delta) t).[trans Delta v/] target /\
+    star lcbv (trans Delta t.[v/]) target.
+Admitted.
+
+Lemma trans_is_value_impure Delta v:
+  is_value v ->
+  impure = is_pure Delta v ->
+  (exists u,
+    trans Delta v = EVariantSome u /\
+    LCValues.is_value u /\
+    exists vv, trans Delta vv = u /\ pure = is_pure Delta vv)
+  \/ trans Delta v = EVariantNone.
+Admitted.
+
+Lemma trans_impure_None Delta t v:
+  trans Delta v = EVariantNone ->
+  star lcbv (trans Delta t.[v/]) EVariantNone.
+(* Alain to Denis: This is the "lemma" we discussed last time for the optimization property. We need to add hypothesis on trans to make sure this is indeed true, as it is not true in general. 
+
+One candidate should be that free variables must make a difference to the computed term.
+
+One other candidate is that terms must be fully applied in some sense.
+
+In both cases, this propertie is not trivial.
+*)
+Admitted.
+
+Definition diagram t1 t2 :=
+  exists target, star lcbv t1 target /\ star lcbv t2 target.
+
+
+Lemma diagram_match_branch_some t2 t2':
+  diagram t2 t2' ->
+  forall u t1,
+  diagram (EMatch u t1 t2) (EMatch u t1 t2').
+Admitted.
+
+Lemma diagram_match_cond u u':
+  diagram u u' ->
+  forall t1 t2,
+  diagram (EMatch u t1 t2) (EMatch u' t1 t2).
+Admitted.
+
+Lemma diagram_app t1 t1':
+  diagram t1 t1' ->
+  forall t2,
+  diagram (EApp t1 t2) (EApp t1' t2).
+Admitted.
+
+Lemma diagram_lift t1 t2:
+  diagram t1 t2 ->
+  forall n,
+  diagram (lift n t1) (lift n t2).
+Admitted.
+
+Lemma is_pure_stable t t':
+  dcbv t t' ->
+  forall Delta,
+  is_pure Delta t = is_pure Delta t'.
+Proof.
+  induction 1; tryfalse; intros; try solve [simpl; eauto].
+  { admit "not true: first we don't have any hypothesis on whenever t or v are pure or not. Moreother, if [t = Lam x], then it is pure. hence u is pure. Disproving the lemma.". }
+  { admit "always true, but we don't have the correct lemma here.". }
+  { admit "always true, but we don't have the correct lemma here.". }
+Abort.
+
+
+
 Lemma trans_correct t1 t2 Gamma T:
   jt Gamma t1 T ->
   forall Delta,
-  no_compile_error (trans Delta t1) ->
   dcbv t1 t2 ->
 
   exists target,
     star lcbv (trans Delta t1) target /\
-    star lcbv (trans Delta t2) target.
+    star lcbv (trans Delta t2) target.  
 Proof.
-  intros Hjt Delta Hcompil Hdcbv.
-  revert Hdcbv Gamma T Hjt Delta Hcompil.
+  intros Hjt Delta Hdcbv.
+  revert Hdcbv Gamma T Hjt Delta.
 
-  induction 1; tryfalse; intros; unpack; try solve [repeat eexists; eauto].
-  * subst; eexists; split.
-    2:{ eapply star_refl. }
+  induction 1; tryfalse.
+  * (* Beta-reduction with [v] a value *)
+    intros.
+    simpl; remember (is_pure Delta v) as p; induction p.
+    { (* [v] is [pure] *)
+      destruct trans_subst_pure with Delta t v as
+        [target [Htarget1 Htarget2]]; eauto.
+      exists target; split.
+      { eapply star_step.
+        { eapply RedBetaV; eauto using trans_is_value. }
+        eauto.
+      } {
+        subst. eauto.
+      }
+    }
+    { (* [v] is [impure] *)
+      unfold monad_bind.
+      destruct trans_is_value_impure with Delta v
+        as [[v' [Hv [Hv'1 [vv [Hv'2 Hv'3]]]]]| Hv]; eauto; rewrite Hv.
+      { (* [v] is [Some v'] *)
+        destruct trans_subst_pure with Delta t vv as
+          [target [Htarget1 Htarget2]]; eauto.
+        exists target; split.
+        { eapply star_step. { eapply RedEMatchSomeV; eauto. }
+          eapply star_step. { eapply RedBetaV; eauto. }
+          asimpl.
+          rewrite <- Hv'2; eauto.
+        }
+        { subst.
+          admit "this i don't really know how to do for now".
+        }
+      }
+      { (* [v] is [None] *)
+        eexists; split.
+        { eapply star_one. { eapply RedEMatchNone; eauto. } }
+        { subst; eapply trans_impure_None; eauto. }
+      }
+    }
+  * (* AppL *)
+    intros.
+    inverts Hjt.
+    edestruct IHHdcbv as [target [Htarget1 Htarget2]]; eauto.
     simpl.
-    induction v; tryfalse.
-    - admit "Variable should not be values. Hence this case should not arise. (Problem in red specification)".
-    - admit "More complicated version of the next case.".
-    - asimpl.
-      eapply star_one.
-      unfold monad_bind, monad_return, monad_empty.
-      eapply RedEMatchSomeV.
-      + trivial.
-      + reflexivity.
-      + unfold LCValues.is_value, LCValues.if_value; simpl.
-        admit "Error: OConst should be a value in LCValues. (specification issue)".
-      + rewrite trans_te_substitution with (Const b .: ids).
-        asimpl; eauto. 
-  * inv jt.
-    assert (no_compile_error (trans Delta t1)). { admit. }
+    (* 8 cases to consider. *)
+    remember (is_pure Delta t1) as p1.
+    remember (is_pure Delta t2) as p2.
+    remember (is_pure Delta u) as p3.
+    induction p1, p2, p3; unfold monad_bind; asimpl.
+    { (* pure, pure, pure *)
+      exists (EApp target (trans Delta u)); split;
+      eapply LCReduction.star_cbv_EAppL; eauto.
+    }
+    { (* pure, pure, impure *)
+      eapply diagram_match_branch_some.
+      eapply diagram_app.
+      eapply diagram_lift.
+      unfold diagram; eauto.
+    }
+    { (* pure, impure, pure *)
+      admit "induction hypothesis is not sufficent to derive this property. Indeed, in the case where [t1 = t2 = App x y], the induction hypothesis indicate [star lcbv (trans Delta t1) (trans Delta t1)]. In this case, we don't have any relationship between [L.EApp (trans Delta t1) (trans Delta u)] and [EMatch (trans Delta t2) EVariantNone (L.EApp (L.EVar 0) (lift 1 (trans Delta u)))].
+      
+      
+      One way to fix this could be to have is_pure is stable relative to dcbv. But this lemma is not true. see above for a tenative of proof".
+    }
+    { (* pure, impure, impure *)
+      admit "same as previous case.".
+    }
+    { (* impure, pure, pure *)
+      admit "same as previous case.".
+    }
+    { (* impure, pure, impure *)
+      admit "same as previous case.".
+    }
+    { (* impure, impure, pure *)
+      eapply diagram_match_cond.
+      unfold diagram; eauto.
+    }
+    { (* impure, impure, impure *)
+      eapply diagram_match_cond.
+      unfold diagram; eauto.
+    }
+  * admit "This should be around the same thing as the previous case.".
+  * simpl.
+    admit "error: if the term is impure, and [trans Delta t] is None, then the left hand side reduces to None while the right hand side reduces to Conflict.".
+  * simpl; intros. 
+    remember (is_pure Delta t) as p; induction p; unfold monad_bind; eexists; split.
+    all: try solve [ eapply star_refl ].
+    eapply star_one.
+    eapply RedEMatchConflict. 
+    all: try solve [ eapply star_one]
 
-    destruct (IHHdcbv _ _ H5 _ H2) as [target [Htarget1 Htarget2]].
-    exists (EApp target (trans Delta u)).
-    split; eapply star_one; asimpl.
-    all: admit.
-  * destruct (IHHdcbv Delta) as [target [Htarget1 Htarget2]].
-    exists (EApp (trans Delta v) target).
-    induction v; simpl in H0; tryfalse.
-    (* v is a value. *)
+
+
 Admitted.
-
